Foundation/Modal/Neighborhood/Logic/EMT4.lean
@@ -26,7 +26,7 @@ instance : Entailment.Consistent Modal.EMT4 := consistent_of_sound_frameclass Fr
   apply Set.mem_setOf_eq.mpr;
   constructor;
 
-instance : Complete Modal.EMT4 FrameClass.EMT4 := complete_of_canonical_frame FrameClass.EMT4 (maximalCanonicalFrame (Modal.EMT4)) $ by
+instance : Complete Modal.EMT4 FrameClass.EMT4 := maximalCanonicalFrame.completeness $ by
   apply Set.mem_setOf_eq.mpr;
   constructor;
 
